ind/Example.fst
@@ -10,7 +10,5 @@ let main () : HST.Stack unit (fun _ -> True) (fun _ _ _ -> True) =
   let d : DLL.dll UInt32.t = DLL.dll_new () in
   let n1 = DLL.node_of 1ul in
   let n2 = DLL.node_of 2ul in
-  let h0 = HST.get () in
-  assume (DLL.fp_node n1 `B.loc_disjoint` DLL.fp_dll h0 d);
   DLL.dll_insert_at_head d n1;
   HST.pop_frame ()
